coq/proof/SoundInfrules.v
@@ -27,12 +27,13 @@ Require Import SoundInfruleTransitivity.
 
 Set Implicit Arguments.
 
-Lemma apply_infrule_sound
+Lemma apply_arithmetic_infrule_sound
       m_src m_tgt
       conf_src st_src
       conf_tgt st_tgt
       invst0 invmem0 inv0
       infrule
+      (ARITHMETIC: Hints.Infrule.is_arithmetic infrule = true)
       (CONF: InvState.valid_conf m_src m_tgt conf_src conf_tgt)
       (STATE: InvState.Rel.sem conf_src conf_tgt st_src st_tgt invst0 invmem0 inv0)
       (MEM: InvMem.Rel.sem conf_src conf_tgt st_src.(Mem) st_tgt.(Mem) invmem0):
@@ -42,60 +43,26 @@ Lemma apply_infrule_sound
     <<MEM: InvMem.Rel.sem conf_src conf_tgt st_src.(Mem) st_tgt.(Mem) invmem1>> /\
     <<MEMLE: InvMem.Rel.le invmem0 invmem1>>.
 Proof.
-  destruct infrule.
-  - ADMIT "add_commutative_tgt".
-  - ADMIT "add_const_not".
-  - ADMIT "add_dist_sub".
-  - ADMIT "add_sub".
-  - ADMIT "add_mask".
-  - ADMIT "add_onebit".
-  - ADMIT "add_or_and".
-  - ADMIT "add_select_zero".
-  - ADMIT "add_select_zero2".
-  - ADMIT "add_shift".
-  - ADMIT "add_signbit".
-  - ADMIT "add_xor_and".
-  - ADMIT "add_zext_bool".
-  - ADMIT "and_de_morgan".
-  - ADMIT "and_mone".
-  - ADMIT "and_not".
-  - ADMIT "and_or".
-  - ADMIT "and_or_const2".
-  - ADMIT "and_same".
-  - ADMIT "and_true_bool".
-  - ADMIT "and_true_bool_tgt".
-  - ADMIT "and_undef".
-  - ADMIT "and_xor_const".
-  - ADMIT "and_zero".
-  - ADMIT "and_or_not1".
-  - ADMIT "bop_associative".
-  - ADMIT "bop_commutative".
-  - ADMIT "bop_commutative_rev".
-  - ADMIT "bop_commutative_tgt".
-  - ADMIT "bop_commutative_rev_tgt".
-  - ADMIT "fbop_commutative".
-  - ADMIT "fbop_commutative_rev".
-  - ADMIT "fbop_commutative_tgt".
-  - ADMIT "fbop_commutative_rev_tgt".
-  - ADMIT "bop_distributive_over_selectinst".
-  - ADMIT "bop_distributive_over_selectinst2".
-  - ADMIT "bitcastptr".
-  - ADMIT "bitcast_bitcast".
-  - ADMIT "bitcast_bitcast_rev_tgt".
-  - ADMIT "bitcast_double_i64".
-  - ADMIT "bitcast_load".
-  - ADMIT "bitcast_fpext".
-  - ADMIT "bitcast_fptosi".
-  - ADMIT "bitcast_fptoui".
-  - ADMIT "bitcast_fptrunc".
-  - ADMIT "bitcast_inttoptr".
-  - ADMIT "bitcast_ptrtoint".
-  - ADMIT "bitcast_sext".
-  - ADMIT "bitcast_sametype".
-  - ADMIT "bitcast_sitofp".
-  - ADMIT "bitcast_trunc".
-  - ADMIT "bitcast_uitofp".
-  - ADMIT "bitcast_zext".
+  ADMIT "we will not prove soundness of arithmetic infrules, Alive (SMT solver) can prove this".
+Qed.
+
+Lemma apply_non_arithmetic_infrule_sound
+      m_src m_tgt
+      conf_src st_src
+      conf_tgt st_tgt
+      invst0 invmem0 inv0
+      infrule
+      (ARITHMETIC: Hints.Infrule.is_arithmetic infrule = false)
+      (CONF: InvState.valid_conf m_src m_tgt conf_src conf_tgt)
+      (STATE: InvState.Rel.sem conf_src conf_tgt st_src st_tgt invst0 invmem0 inv0)
+      (MEM: InvMem.Rel.sem conf_src conf_tgt st_src.(Mem) st_tgt.(Mem) invmem0):
+  exists invst1 invmem1,
+    <<STATE: InvState.Rel.sem conf_src conf_tgt st_src st_tgt invst1 invmem1
+                              (Infrules.apply_infrule m_src m_tgt infrule inv0)>> /\
+    <<MEM: InvMem.Rel.sem conf_src conf_tgt st_src.(Mem) st_tgt.(Mem) invmem1>> /\
+    <<MEMLE: InvMem.Rel.le invmem0 invmem1>>.
+Proof.
+  destruct infrule; compute in ARITHMETIC; try (by contradict ARITHMETIC).
   - (* diffblock_unique *)
     exists invst0, invmem0. splits; eauto; [|reflexivity].
     ss. des_ifs.
@@ -114,19 +81,6 @@ Proof.
   - ADMIT "!diffblock_global_global".
   - ADMIT "!diffblock_lessthan".
   - ADMIT "!diffblock_noalias".
-  - ADMIT "fadd_commutative_tgt".
-  - ADMIT "fbop_distributive_over_selectinst".
-  - ADMIT "fbop_distributive_over_selectinst2".
-  - ADMIT "fmul_commutative_tgt".
-  - ADMIT "fpext_bitcast".
-  - ADMIT "fpext_fpext".
-  - ADMIT "fptosi_bitcast".
-  - ADMIT "fptosi_fpext".
-  - ADMIT "fptoui_bitcast".
-  - ADMIT "fptoui_fpext".
-  - ADMIT "fptrunc_bitcast".
-  - ADMIT "fptrunc_fpext".
-  - ADMIT "gepzero".
   -
     exists invst0, invmem0. splits; eauto; [|reflexivity].
     inv STATE. econs; eauto. ss.
@@ -159,105 +113,6 @@ Proof.
    unfold Debug.debug_string, Debug.debug_print2 in H;
      apply LESSDEF; auto.
    admit. admit. admit. admit. admit. admit.
-  - ADMIT "gep_inbounds_add".
-  - ADMIT "inttoptr_bitcast".
-  - ADMIT "inttoptr_ptrtoint".
-  - ADMIT "inttoptr_zext".
-  - ADMIT "inttoptr_load".
-  - (* lessthan_undef *)
-    admit.
-  - (* lessthan_undef_tgt *)
-    admit.
-  - (* lessthan_undef_const *)
-    (* exists invst0, invmem0. splits; eauto; [|reflexivity]. *)
-    (* destruct c eqn:C; (try destruct floating_point5); *)
-    (*   (try (inv STATE; econs; eauto; *)
-    (*   ss; inv SRC; econs; eauto; ss; *)
-    (*   ii; apply Exprs.ExprPairSetFacts.add_iff in H; des)); *)
-    (* (try (subst; esplits; ss; eauto; *)
-    (*   eapply all_undef_lessdef_aux; apply const2GV_undef in VAL1; des; eauto; *)
-    (*   unfold flatten_typ in VAL1; simpl in VAL1; destruct (CurTargetData conf_src); *)
-  (*     inv VAL1; eauto)); (try (eapply LESSDEF; auto)). *)
-    admit.
-  - (* lessthan_undef_const_tgt *)
-    admit.
-    (* exists invst0, invmem0. splits; eauto; [|reflexivity]. *)
-    (* destruct c eqn:C; (try destruct floating_point5); *)
-    (*   (try (inv STATE; econs; eauto; *)
-    (*   ss; inv TGT; econs; eauto; ss; *)
-    (*   ii; apply Exprs.ExprPairSetFacts.add_iff in H; des)); *)
-    (* (try (subst; esplits; ss; eauto; *)
-    (*   eapply all_undef_lessdef_aux; apply const2GV_undef in VAL1; des; eauto; *)
-    (*   unfold flatten_typ in VAL1; simpl in VAL1; destruct (CurTargetData conf_tgt); *)
-    (*     inv VAL1; eauto)); (try (eapply LESSDEF; auto)). *)
-  - admit.
-    (* ADMIT "lessthan_undef_const_gep_or_cast" *)
-  - ADMIT "mul_bool".
-  - ADMIT "mul_mone".
-  - ADMIT "mul_neg".
-  - ADMIT "mul_shl".
-  - ADMIT "neg_val".
-  - ADMIT "or_and".
-  - ADMIT "or_and_xor".
-  - ADMIT "or_commutative_tgt".
-  - ADMIT "or_false".
-  - ADMIT "or_false_tgt".
-  - ADMIT "or_mone".
-  - ADMIT "or_not".
-  - ADMIT "or_or ".
-  - ADMIT "or_or2 ".
-  - ADMIT "or_same".
-  - ADMIT "or_undef".
-  - ADMIT "or_xor".
-  - ADMIT "or_xor2".
-  - ADMIT "or_xor3".
-  - ADMIT "or_xor4".
-  - ADMIT "or_zero".
-  - ADMIT "ptrtoint_bitcast".
-  - ADMIT "ptrtoint_inttoptr".
-  - ADMIT "ptrtoint_load".
-  - ADMIT "ptrtoint_zero".
-  - ADMIT "!replace_rhs".
-  - ADMIT "!replace_rhs_opt".
-  - ADMIT "rem_neg".
-  - ADMIT "sdiv_mone".
-  - ADMIT "sdiv_sub_srem".
-  - ADMIT "select_icmp_eq".
-  - ADMIT "select_icmp_eq_xor1".
-  - ADMIT "select_icmp_eq_xor2".
-  - ADMIT "select_icmp_ne".
-  - ADMIT "select_icmp_ne_xor1".
-  - ADMIT "select_icmp_ne_xor2".
-  - ADMIT "select_icmp_sgt_const".
-  - ADMIT "select_icmp_sgt_xor1".
-  - ADMIT "select_icmp_sgt_xor2".
-  - ADMIT "select_icmp_slt_const".
-  - ADMIT "select_icmp_slt_xor1".
-  - ADMIT "select_icmp_slt_xor2".
-  - ADMIT "select_icmp_slt_one".
-  - ADMIT "select_icmp_ugt_const".
-  - ADMIT "select_icmp_ult_const".
-  - ADMIT "sext_bitcast".
-  - ADMIT "sext_sext".
-  - ADMIT "sext_trunc_ashr".
-  - ADMIT "sext_zext".
-  - ADMIT "shift_undef1".
-  - ADMIT "shift_undef2".
-  - ADMIT "shift_zero1".
-  - ADMIT "shift_zero2".
-  - ADMIT "sitofp_bitcast".
-  - ADMIT "sitofp_sext".
-  - ADMIT "sitofp_zext".
-  - ADMIT "sub_add".
-  - ADMIT "sub_const_add".
-  - ADMIT "sub_const_not".
-  - ADMIT "sub_mone".
-  - ADMIT "sub_onebit".
-  - ADMIT "sub_or_xor".
-  - ADMIT "sub_remove".
-  - ADMIT "sub_sdiv".
-  - ADMIT "sub_sub".
-  - ADMIT "sub_shl".
   - (* transitivity *)
     exists invst0, invmem0. splits; eauto; [|reflexivity].
     ss.
@@ -433,15 +288,6 @@ Proof.
       eapply Exprs.ExprPairSetFacts.mem_iff; eauto.
       eapply Exprs.ExprPairSetFacts.add_iff; eauto.
     }
-  - ADMIT "trunc_onebit".
-  - ADMIT "trunc_zext".
-  - ADMIT "trunc_sext".
-  - ADMIT "trunc_bitcast".
-  - ADMIT "trunc_ptrtoint".
-  - ADMIT "trunc_trunc".
-  - ADMIT "trunc_trunc_rev_tgt".
-  - ADMIT "trunc_load_bitcast_rev_tgt".
-  - ADMIT "trunc_load_const_bitcast_rev_tgt".
   - (* substitute *)
     exists invst0, invmem0.
     esplits; eauto; [ | reflexivity ].
@@ -469,23 +315,6 @@ Proof.
     intro LD; des. clear Heq.
     inv STATE. clear - TGT LD.
     eapply substitute_spec_unary; eauto.
-  - ADMIT "udiv_sub_urem".
-  - ADMIT "udiv_zext".
-  - ADMIT "udiv_zext_const".
-  - ADMIT "uitofp_bitcast".
-  - ADMIT "uitofp_zext".
-  - ADMIT "urem_zext".
-  - ADMIT "urem_zext_const".
-  - ADMIT "xor_commutative_tgt".
-  - ADMIT "xor_not".
-  - ADMIT "xor_same".
-  - ADMIT "xor_undef".
-  - ADMIT "xor_zero".
-  - ADMIT "zext_bitcast".
-  - ADMIT "zext_trunc_and".
-  - ADMIT "zext_trunc_and_xor".
-  - ADMIT "zext_xor".
-  - ADMIT "zext_zext".
   - ADMIT "!intro_ghost_src".
   - ss. des_ifs; cycle 1.
     { esplits; eauto. reflexivity. }
@@ -628,74 +457,28 @@ Proof.
     ii. apply Exprs.ExprPairSetFacts.add_iff in H. des.
     + subst. esplits; eauto. apply GVs.lessdef_refl.
     + eapply LESSDEF; eauto.
-  - ADMIT "icmp_inverse".
-  - ADMIT "icmp_inverse_rhs".
-  - ADMIT "icmp_inverse_tgt".
-  - ADMIT "icmp_inverse_rhs_tgt".
-  - ADMIT "icmp_swap_operands".
-  - ADMIT "icmp_swap_operands_rev".
-  - ADMIT "icmp_swap_operands_tgt".
-  - ADMIT "icmp_swap_operands_rev_tgt".
-  - ADMIT "fcmp_swap_operands".
-  - ADMIT "fcmp_swap_operands_rev".
-  - ADMIT "fcmp_swap_operands_tgt".
-  - ADMIT "fcmp_swap_operands_rev_tgt".
-  - ADMIT "icmp_eq_add_add".
-  - ADMIT "icmp_eq_same".
-  - ADMIT "icmp_eq_same_tgt".
-  - ADMIT "icmp_eq_sub_sub".
-  - ADMIT "icmp_eq_xor_not".
-  - ADMIT "icmp_eq_xor_xor".
-  - ADMIT "icmp_eq_sub".
-  - ADMIT "icmp_eq_srem".
-  - ADMIT "icmp_ne_add_add".
-  - ADMIT "icmp_ne_sub".
-  - ADMIT "icmp_ne_sub_sub".
-  - ADMIT "icmp_ne_srem".
-  - ADMIT "icmp_ne_xor".
-  - ADMIT "icmp_ne_xor_xor".
-  - ADMIT "icmp_neq_same".
-  - ADMIT "icmp_neq_same_tgt".
-  - ADMIT "icmp_sge_or_not".
-  - ADMIT "icmp_sgt_and_not".
-  - ADMIT "icmp_sle_or_not".
-  - ADMIT "icmp_slt_and_not".
-  - ADMIT "icmp_uge_or_not".
-  - ADMIT "icmp_ugt_and_not".
-  - ADMIT "icmp_ule_or_not".
-  - ADMIT "icmp_ult_and_not".
   - ADMIT "!implies_false".
-  - (* remove_maydiff *)
-    exists invst0, invmem0. splits; eauto. reflexivity.
-    (* remove it *)
-  - (* remove_maydiff_rhs *)
-    exists invst0, invmem0. splits; eauto. reflexivity.
-    (* remove it *)
-  - ADMIT "!stash_variable".
-  - ADMIT "add_mul_fold".
-  - ADMIT "add_distributive".
-  - ADMIT "rem_neg2".
-  - ADMIT "select_trunc".
-  - ADMIT "select_add".
-  - ADMIT "select_const_gt".
-  - ADMIT "cmp_eq_sub".
-  - ADMIT "cmp_ne_sub".
-  - ADMIT "cmp_eq_srem".
-  - ADMIT "cmp_eq_srem2".
-  - ADMIT "cmp_ne_srem".
-  - ADMIT "cmp_ne_srem2".
-  - ADMIT "cmp_eq_xor".
-  - ADMIT "cmp_ne_xor".
 Admitted.
 
-(*  ADMIT "Infrule
-We will not prove soundness of infrules in this submission.
-All the infrules are simple, and we carefully installed it, so it is less likely to introduce a bug.
-Also, even in case some infrules contain bugs, the bugs does not affect the whole system,
-and it should be easy to fix. Moreover, we did prove most of the infrules in the former version of simplberry.
-To our experience, proving infrules can be done withn reasonable amount of engineering effort (maybe 2 weeks)
-by using automation techniques. However, we skip it for now.".
-Qed.*)
+Lemma apply_infrule_sound
+      m_src m_tgt
+      conf_src st_src
+      conf_tgt st_tgt
+      invst0 invmem0 inv0
+      infrule
+      (CONF: InvState.valid_conf m_src m_tgt conf_src conf_tgt)
+      (STATE: InvState.Rel.sem conf_src conf_tgt st_src st_tgt invst0 invmem0 inv0)
+      (MEM: InvMem.Rel.sem conf_src conf_tgt st_src.(Mem) st_tgt.(Mem) invmem0):
+  exists invst1 invmem1,
+    <<STATE: InvState.Rel.sem conf_src conf_tgt st_src st_tgt invst1 invmem1
+                              (Infrules.apply_infrule m_src m_tgt infrule inv0)>> /\
+    <<MEM: InvMem.Rel.sem conf_src conf_tgt st_src.(Mem) st_tgt.(Mem) invmem1>> /\
+    <<MEMLE: InvMem.Rel.le invmem0 invmem1>>.
+Proof.
+  destruct (Hints.Infrule.is_arithmetic infrule) eqn:T; ss.
+  - eapply apply_arithmetic_infrule_sound; eauto.
+  - eapply apply_non_arithmetic_infrule_sound; eauto.
+Qed.
 
 Lemma apply_infrules_sound
       m_src m_tgt
